# Exercises 03: Z Transform

::: {.hidden}
$$
\newcommand{\underuparrow}[1]{\underset{\uparrow}{#1}}$$
$$
:::

## Exercise 1

Compute the convolution of the signals:
$x_1[n] = \{ ...,0,1,2,\underuparrow{3},4,0,...\}$ and $x_2[n] = \{...,0,2,\underuparrow{2},3,3,0,...\}$

- a). using the Z transform

- b). as a product of polynomials

### Solution {.unnumbered}

a). *Using the Z transform*

We can write the convolution as a product of the Z transforms of the two signals:
$$x_1[n] \leftrightarrow X_1(z) = 1z^2 + 2z^1 + 3 + 4z^{-1}$$
$$x_2[n] \leftrightarrow X_2(z) = 2z^1 + 2 + 3z^{-1} + 3z^{-2}$$
$$\begin{aligned}
x_1[n] \ast x_2[n] \leftrightarrow X_1 \cdot X_2(z) &= (1z^2 + 2z^1 + 3 + 4z^{-1}) \cdot (2z^1 + 2 + 3z^{-1} + 3z^{-2}) \\
&= 2z^3 + 6z^2 + 13z + 23 + 23z^{-1} + 21z^{-2} + 12z^{-3} \\
&= \{2, 6, 13, \underuparrow{23}, 23, 21, 12\} \\
\end{aligned}
$$

b). *As a product of polynomials*

The Z transform is simply associating a polynomial to a signal, according
to some rules (variable is $z$, powers are in decreasing order).
Convolution is a polynomial multiplication, irrespective of how
we define the polynomials (like in Z transform, or in some other way).


We could also associate any polynomials and compute the convolution
as a product of those polynomials.
$$\{1, 2, 3, 4\} \rightarrow 1 + 2X + 3X^2 + 4X^3$$
$$\{2, 2, 3, 3\} \rightarrow 2 + 2X + 3X^2 + 3X^3$$
$$\begin{aligned}
x_1[n] \ast x_2[n] &\rightarrow (1 + 2X + 3X^2 + 4X^3) \cdot (2 + 2X + 3X^2 + 3X^3) \\
&= 2 + 6X + 13X^2 + 23X^3 + 23X^4 + 21X^5 + 12X^6 \\
&= \{2, 6, 13, 23, 23, 21, 12\} \\
\end{aligned}$$

The origin of time is at the element containing the product of the two values at the origin of time in the two input signals, i.e. $3X^2$ from $x_1[n]$ and $2X$ from $x_2[n]$ is $6X^3$, so it's the element with $X^3$ in the output signal.

## Exercise 2

Find the Z transform of the following signals:

- a). $$x[n] = \left( \frac{1}{3} \right)^n u[n]$$

- b). $$x[n] = \begin{cases}
	\left( \frac{1}{3} \right)^n, & n \geq 0 \\
	\left( \frac{1}{2} \right)^{-n}, & n < 0
	\end{cases}$$

- c). $$x[n] = \left( \frac{1}{2} \right)^n \sin (\frac{\pi}{3}n) u[n]$$

### Solution {.unnumbered}

a). We use the definition of the Z transform:
$$X(z) = \sum_{n=-\infty}^{\infty} x[n] z^{-n}$$

In our case, $x[n] = \left( \frac{1}{3} \right)^n u[n]$, so it has
only zeros on the left side, because of $u[n]$.
Therefore we only need to sum
from $n=0$ to $\infty$:
$$\begin{aligned}
X(z) &= \sum_{n=0}^{\infty} x[n] z^{-n} \\
&= \sum_{n=0}^{\infty} \left( \frac{1}{3} \right)^n z^{-n} \\
&= \sum_{n=0}^{\infty} \left( \frac{1}{3z} \right)^n \\
\end{aligned}$$

Denoting $q = \frac{1}{3z}$, we have here the sum of a geometric series:
$$X(z) = \sum_{n=0}^{\infty} q^n  = 1 + q + q^2 +...$$

It is known that the sum of a geometric series with element $q$ is:
$$\sum_{n=0}^{\infty} q^n = \frac{1}{1-q}$$
if $|q| < 1$. The sum in infinite otherwise ($|q| \geq 1$).

Therefore in our case, $q = \frac{1}{3z}$, so if
we have $|\frac{1}{3z}| < 1$, the sum is:
$$X(z) = \frac{1}{1-q} = \frac{1}{1-\frac{1}{3z}} = \frac{3z}{3z-1} = \frac{z}{z-\frac{1}{3}}$$

The condition $|\frac{1}{3z}| < 1$ defines the Region of Convergence (ROC).
We can more conveniently write it as:
$$|\frac{1}{3z}| < 1 \rightarrow |z| > \frac{1}{3}$$

Therefore the answer is:
$$X(z) = \frac{z}{z-\frac{1}{3}}, \quad \text{ROC:}|z| > \frac{1}{3}$$

b). We use the definition of the Z transform, but now we also have
values on the left side of $x[n]$. We split the sum in two parts:
$$\begin{aligned}
X(z) &= \sum_{n=-\infty}^{\infty} x[n] z^{-n} \\
&= \sum_{n=-\infty}^{-1} x[n] z^{-n} + \sum_{n=0}^{\infty} x[n] z^{-n} \\
&= \sum_{n=-\infty}^{-1} \left( \frac{1}{2} \right)^{-n} z^{-n} + \sum_{n=0}^{\infty} \left( \frac{1}{3} \right)^n z^{-n} \\
&= \sum_{n=-\infty}^{-1} \left( \frac{z}{2} \right)^{-n} + \sum_{n=0}^{\infty} \left( \frac{1}{3z} \right)^n \\
\end{aligned}$$

The second sum is similar to the one in the previous exercise, so
it results in:
$$\sum_{n=0}^{\infty} \left( \frac{1}{3z} \right)^n = \frac{z}{z-\frac{1}{3}}
\quad \text{if} \quad |z| > \frac{1}{3}$$

The first sum is also a geometric series. First, we can do a variable change
$n = -m$, so that we have a sum from $m=1$ to $\infty$ instead:
$$\sum_{n=-\infty}^{-1} \left( \frac{z}{2} \right)^{-n} = \sum_{m=1}^{\infty} \left( \frac{z}{2} \right)^{m}$$

This is a geometric series with element $q = \frac{z}{2}$, but the first
element $q^0 = 1$ is missing, so we have to remove it from the sum:
$$\begin{aligned}
\sum_{m=1}^{\infty} \left( \frac{z}{2} \right)^{m} &= \sum_{m=0}^{\infty} \left( \frac{z}{2} \right)^{m} - 1 \\
&= \frac{1}{1-\frac{z}{2}} - 1 \\
&= \frac{1}{1-\frac{z}{2}} - \frac{1-\frac{z}{2}}{1-\frac{z}{2}} \\
&= \frac{\frac{z}{2}}{1-\frac{z}{2}} \\
&= - \frac{z}{z-2}
\end{aligned}$$

The condition is $|\frac{z}{2}| < 1$, which is equivalent to $|z| < 2$.

Adding the two sums, we have:
$$\begin{aligned}
X(z) &= - \frac{z}{z-2} + \frac{z}{z-\frac{1}{3}} \\
&= \frac{-z(z-\frac{1}{3}) + z(z-2)}{(z-2)(z-\frac{1}{3})} \\
&= \frac{-\frac{5}{3}z}{(z-2)(z-\frac{1}{3})} \\
\end{aligned}$$

The ROC is the intersection of the ROCs of the two sums, which is:
$$\text{ROC:} \quad |z| > \frac{1}{3} \quad \text{and} \quad |z| < 2$$
$$\text{ROC:} \quad \frac{1}{3} < |z| < 2$$

c). We can write the $\sin$ using the Euler formula:
$$\sin(x) = \frac{e^{jx} - e^{-jx}}{2j}$$
$$\sin (\frac{\pi}{3}n) = \frac{e^{j\frac{\pi}{3}n} - e^{-j\frac{\pi}{3}n}}{2j}$$

The $u[n]$ cancels the left part of the signal, so the Z transform sum starts from 0:
$$\begin{aligned}
X(z) &= \sum_{n=0}^{\infty} \left( \frac{1}{2} \right)^n \frac{e^{j\frac{\pi}{3}n} - e^{-j\frac{\pi}{3}n}}{2j} z^{-n} \\
&= \frac{1}{2j} \sum_{n=0}^{\infty} \left( \frac{e^{j\frac{\pi}{3}}}{2z} \right)^n - \frac{1}{2j} \sum_{n=0}^{\infty} \left( \frac{e^{-j\frac{\pi}{3}}}{2z} \right)^n \\
\end{aligned}$$
(since $e^{j\frac{\pi}{3}n} = (e^{j\frac{\pi}{3}})^n$).

From now on, we use the same geometric series formula:
$$\frac{1}{2j} \sum_{n=0}^{\infty} \left( \frac{e^{j\frac{\pi}{3}}}{2z} \right)^n = \frac{1}{2j} \frac{1}{1 - q} = \frac{1}{2j} \frac{1}{1 - \frac{e^{j\frac{\pi}{3}}}{2z}}$$
$$\frac{1}{2j} \sum_{n=0}^{\infty} \left( \frac{e^{-j\frac{\pi}{3}}}{2z} \right)^n = \frac{1}{2j} \frac{1}{1 - q} = \frac{1}{2j} \frac{1}{1 - \frac{e^{-j\frac{\pi}{3}}}{2z}}$$
with the conditions $|\frac{e^{j\frac{\pi}{3}}}{2z}| < 1$ and $|\frac{e^{-j\frac{\pi}{3}}}{2z}| < 1$, which are equivalent to $|z| > \frac{1}{2}$.

Adding the two sums, we have:
$$\begin{aligned}
X(z) &= \frac{1}{2j} \frac{1}{1 - \frac{e^{j\frac{\pi}{3}}}{2z}} - \frac{1}{2j} \frac{1}{1 - \frac{e^{-j\frac{\pi}{3}}}{2z}} \\
&= \frac{1}{2j} \frac{\frac{e^{j\frac{\pi}{3}} - e^{-j\frac{\pi}{3}}}{2z}}{(1 - \frac{e^{j\frac{\pi}{3}}}{2z})(1 - \frac{e^{-j\frac{\pi}{3}}}{2z})} \\
&= \frac{\frac{1}{2z}\sin(\frac{\pi}{3})}{(1 - \frac{e^{j\frac{\pi}{3}}}{2z})(1 - \frac{e^{-j\frac{\pi}{3}}}{2z})} \\
&= \frac{\sin(\frac{\pi}{3})}{(2z - e^{j\frac{\pi}{3}})(2z - e^{-j\frac{\pi}{3}})} \\
&= \frac{\sin(\frac{\pi}{3})}{4z^2 - 2ze^{j\frac{\pi}{3}} - 2ze^{-j\frac{\pi}{3}} + 1} \\
&= \frac{\sin(\frac{\pi}{3})}{4z^2 - 2z(e^{j\frac{\pi}{3}} + e^{-j\frac{\pi}{3}}) + 1} \\
&= \frac{\sin(\frac{\pi}{3})}{4z^2 - 2z(2\cos(\frac{\pi}{3})) + 1} \\
&= \frac{\sin(\frac{\pi}{3})}{4z^2 - 4\cos(\frac{\pi}{3})z + 1} \\
&= \frac{\frac{\sqrt{3}}{2}}{4z^2 - 2z + 1} \\
&= \frac{\sqrt{3}}{8} \frac{1}{z^2 - \frac{1}{2}z + \frac{1}{4}} \\
\end{aligned}$$
$$\text{ROC:} \quad |z| > \frac{1}{2}$$


## Exercise 3

Find all the signals $x[n]$ which have the Z transform
$$X(z) = \frac{7}{(1 - 2z^{-1})(1+0.5z^{-1})}$$

### Solution {.unnumbered}

Because we don't specify the ROC, we will have
multiple signals which have the same expression of the Z transform, but with different ROCs.

We find the **inverse Z transform** by using the partial fraction expansion.

First we get rid of the negative powers of $z$, to make calculations easier:
$$X(z) = \frac{7}{(1 - 2z^{-1})(1+0.5z^{-1})} = \frac{7z^2}{(z - 2)(z+0.5)}$$

Then we write $X(z)/z$:
$$\frac{X(z)}{z} = \frac{7z}{(z - 2)(z+0.5)}$$

Then we write the partial fractions:
$$\frac{X(z)}{z} = \frac{7z}{(z - 2)(z+0.5)} = \frac{A}{z-2} + \frac{B}{z+0.5}$$

We can find $A$ and $B$ now, or leave them for later.
$$A = \frac{7z}{z+0.5} \Big|_{z=2} = \frac{7 \cdot 2}{2 + 0.5} = \frac{14}{2.5}$$
$$B = \frac{7z}{z-2} \Big|_{z=-0.5} = \frac{7 \cdot (-0.5)}{-0.5 - 2} = \frac{-3.5}{-2.5}$$

Next we multiply back with $z$:
$$X(z) = A \frac{z}{z-2} + B \frac{z}{z+0.5}$$

Now we use the inverse Z transform table to invert the partial fractions:
$$\begin{aligned}
a^n u[n] &\leftrightarrow \frac{z}{z-a}, \text{ for } |z| > |a| \\
-a^n u[-n-1] &\leftrightarrow \frac{z}{z-a}, \text{ for } |z| < |a| \\
\end{aligned}$$

Because the ROC is not specified, we will have multiple possible signals
for each of the partial fractions.

1. **Case 1**: if $|z| < 0.5 < 2$, we use the variant with $u[-n-1]$ for both fractions:
   $$\begin{aligned}
    \frac{z}{z-2} &\leftrightarrow -2^n u[-n-1] \\
    \frac{z}{z+0.5} &\leftrightarrow -(-0.5)^n u[-n-1]
    \end{aligned}$$
    Therefore the signal is:
    $$x_1[n] = - \frac{14}{2.5} 2^n u[-n-1] - \frac{3.5}{2.5} (-0.5)^n u[-n-1]$$

2. **Case 2**: if $0.5 < |z| < 2$, we use the variant with $u[n]$ for the fraction with $0.5$ and $u[-n-1]$ for the fraction with $2$:
   $$\begin{aligned}
    \frac{z}{z-2} &\leftrightarrow -2^n u[-n-1] \\
    \frac{z}{z+0.5} &\leftrightarrow (-0.5)^n u[n]
    \end{aligned}$$
    Therefore the signal is:
    $$x_2[n] = - \frac{14}{2.5} 2^n u[-n-1] + \frac{3.5}{2.5} (-0.5)^n u[n]$$

3. **Case 3**: if $|z| > 2 > 0.5$, we use the variant with $u[n]$ for both fractions:
   $$\begin{aligned}
   \frac{z}{z-2} &\leftrightarrow 2^n u[n] \\
    \frac{z}{z+0.5} &\leftrightarrow (-0.5)^n u[n]
    \end{aligned}$$
    Therefore the signal is:
    $$x_3[n] = \frac{14}{2.5} 2^n u[n] + \frac{3.5}{2.5} (-0.5)^n u[n]$$

## Exercise 4

Consider the system with the following system equation:
$$y[n] = -0.1 y[n-1] + 0.2 y[n-2] + x[n] + x[n-1]$$

- a). Find the system function H(z), draw the pole-zero diagram, and specify if the system is stable
- b). Compute the impulse response $h[n]$ of the system
- c). Compute the response of the system to the unit step $x[n] = u[n]$
- d). Compute the response of the system to the input signal $x[n] = \left(\frac{1}{3}\right)^n u[n]$

### Solution {.unnumbered}

a). *Find the system function H(z), draw the pole-zero diagram, and specify if the system is stable*

We can find H(z) by taking the Z transform of the system equation:
$$\begin{aligned}
Y(z) &= -0.1 z^{-1} Y(z) + 0.2 z^{-2} Y(z) + X(z) + z^{-1} X(z) \\
Y(z) (1 + 0.1 z^{-1} - 0.2 z^{-2}) &= X(z) (1 + z^{-1}) \\
H(z) = \frac{Y(z)}{X(z)} &= \frac{1 + z^{-1}}{1 + 0.1 z^{-1} - 0.2 z^{-2}} \\
&= \frac{z(z + 1)}{z^2 + 0.1 z - 0.2} \\
\end{aligned}$$

::: {.callout-tip}
#### Quick way of writing $H(z)$

The coefficients of $x[n-k]$ are the coefficients $b_k$ at the numerator of $H(z)$. Here, they are $b_0 = 1$ and $b_1 = 1$.

The coefficients of $y[n-k]$ are the coefficients $a_k$ at the denominator of $H(z)$, **with the opposite sign**. Here, they are $a_1 = 0.1$ and $a_2 = -0.2$ (note the different sign from how they appear in the equation).

Therefore $H(z)$ is:
$$H(z) = \frac{1 + z^{-1}}{1 + 0.1 z^{-1} - 0.2 z^{-2}}$$
:::

Find the zeros as the roots of the numerator polynomial:
$$z(z + 1) = 0 \rightarrow z_1 = 0, \quad z_2 = -1$$
Find the poles as the roots of the denominator polynomial:
$$z^2 + 0.1 z^ - 0.2 = 0 \rightarrow p_1 = -0.5, \quad p_2 = 0.4$$

The pole-zero diagram is:

![Pole-zero diagram](./img/Ex03_04_01.png){width=75%}

The system is stable, because:

- The system is causal, because the system equation is causal (no $y[n+k]$
or $x[n+k]$ terms).
- A causal system is stable if all the poles are inside the unit circle. In our case, the poles are $p_1 = -0.5$ and $p_2 = 0.4$, so they are indeed inside the unit circle.

b). *Compute the impulse response $h[n]$ of the system*

The impulse response $h[n]$ is the inverse Z transform of the system function $H(z)$. We use the same method for inverting the Z transform with partial fractions as in a previous exercise.

We start from the expression of $H(z)$, with positive exponents:
$$H(z) = \frac{z(z + 1)}{z^2 + 0.1 z - 0.2}= \frac{z(z+1)}{(z+0.5)(z-0.4)}$$
Then we write $H(z)/z$:
Write $H(z)/z$:
$$\frac{H(z)}{z} = \frac{z + 1}{(z+0.5)(z-0.4)}$$
Then decompose in partial fractions:
$$\frac{H(z)}{z} = \frac{z + 1}{(z+0.5)(z-0.4)} = \frac{A}{z+0.5} + \frac{B}{z-0.4}$$
Multiply back with $z$:
$$H(z) = A \frac{z}{z+0.5} + B \frac{z}{z-0.4}$$

We know the system is causal, so we know $h[n]$ must be causal, so we invert the fractions using the variant with $u[n]$ for both:
$$\begin{aligned}
\frac{z}{z+0.5} &\leftrightarrow (-0.5)^n u[n] \\
\frac{z}{z-0.4} &\leftrightarrow (0.4)^n u[n]
\end{aligned}$$

The result is:
$$h[n] = A (-0.5)^n u[n] + B (0.4)^n u[n]$$
where $A$ and $B$ are:
$$A = \frac{z+1}{z-0.4} \Big|_{z=-0.5} = \frac{-0.5+1}{-0.5-0.4} = \frac{0.5}{-0.9}$$
$$B = \frac{z+1}{z+0.5} \Big|_{z=0.4} = \frac{0.4+1}{0.4+0.5} = \frac{1.4}{0.9}$$

c). *Compute the response of the system to the unit step $x[n] = u[n]$*

If the system function is $H(z)$, and the input has the Z transform $X(z)$, then the output Z transform is:
$$Y(z) = H(z) X(z)$$

In our case, the input is $x[n] = u[n]$, so its Z transform is:
$$X(z) = \frac{1}{1 - z^{-1}} = \frac{z}{z-1}, \quad \text{ROC:} \quad |z| > 1$$

Therefore:
$$\begin{aligned}
Y(z) &= H(z) X(z) \\
&= \frac{z(z+1)}{(z+0.5)(z-0.4)} \cdot \frac{z}{z-1} \\
&= \frac{z^2(z+1)}{(z+0.5)(z-0.4)(z-1)} \\
\end{aligned}$$

Now we use the same inverse Z procedure as in the previous exercises.

Write $Y(z)/z$, then decompose in partial fractions:
$$\frac{Y(z)}{z} = \frac{z(z+1)}{(z+0.5)(z-0.4)(z-1)} = \frac{A}{z+0.5} + \frac{B}{z-0.4} + \frac{C}{z-1}$$
Multiply back with $z$:
$$Y(z) = A \frac{z}{z+0.5} + B \frac{z}{z-0.4} + C \frac{z}{z-1}$$

The system is causal, the input is causal ($u[n]$), so the output must be causal, so we invert using the variant with $u[n]$ for all fractions:
$$y[n] = A (-0.5)^n u[n] + B (0.4)^n u[n] + C u[n]$$
where $A$, $B$ and $C$ are:
$$A = \frac{z(z+1)}{(z-0.4)(z-1)} \Big|_{z=-0.5} = \frac{-0.5(-0.5+1)}{(-0.5-0.4)(-0.5-1)} = ...$$
$$B = \frac{z(z+1)}{(z+0.5)(z-1)} \Big|_{z=0.4} = \frac{0.4(0.4+1)}{(0.4+0.5)(0.4-1)} = ...$$
$$C = \frac{z(z+1)}{(z+0.5)(z-0.4)} \Big|_{z=1} = \frac{1(1+1)}{(1+0.5)(1-0.4)} = ...$$
and the ROC is the intersection of the ROCs of the three fractions, which is:
$$\text{ROC:} \quad |z| > |-0.5| \quad \text{and} \quad |z| > |0.4| \quad \text{and} \quad |z| > |1|$$
which means:
$$\text{ROC:} \quad |z| > 1$$

d). *Compute the response of the system to the input signal $x[n] = \left(\frac{1}{3}\right)^n u[n]$*

The Z tranform of the input is:
$$X(z) = \frac{1}{1 - \frac{1}{3} z^{-1}} = \frac{z}{z-\frac{1}{3}}, \quad \text{ROC:} \quad |z| > \frac{1}{3}$$

We solve in the same manner as in c).

## Exercise 5

A causal LTI system has the property that if the input signal is
$$x[n] = \left( \frac{1}{3} \right)^n u[n] - \frac{1}{4} \left( \frac{1}{3} \right)^n u[n-1],$$
then the output signal is
$$y[n] = \left( \frac{1}{4} \right)^n u[n]$$

- a). Find the system function H(z), draw the pole-zero diagram
- b). Compute the impulse response $h[n]$ of the system
- c). Find the difference equation of the system
- d). Characterize the system with respect to:

  - length of impulse response (FIR or IIR)
  - implementation (recursive or non-recursive)
  - stability

### Solution {.unnumbered}

a). *Find the system function H(z), draw the pole-zero diagram*

We know that $H(z) = \frac{Y(z)}{X(z)}$. We find $X(z)$ and $Y(z)$, then we divide them to obtain $H(z)$.

For the Z transform of the input, we take each term:
$$\left(\frac{1}{3}\right)^n u[n] \leftrightarrow \frac{z}{z-\frac{1}{3}}, \quad \text{ROC:} \quad |z| > \frac{1}{3}$$
For the second term, observe that we can write it as:
$$\frac{1}{4} \left( \frac{1}{3} \right)^n u[n-1] = \frac{1}{4} \cdot \frac{1}{3} \cdot \left( \frac{1}{3} \right)^{n-1} u[n-1]$$
and $\left( \frac{1}{3} \right)^{n-1} u[n-1]$ is the shifted version of $\left( \frac{1}{3} \right)^n u[n]$, so its Z transform is multiplied by $z^{-1}$:
$$\left( \frac{1}{3} \right)^{n-1} u[n-1] \leftrightarrow z^{-1} \frac{z}{z-\frac{1}{3}}, \quad \text{ROC:} \quad |z| > \frac{1}{3}$$
Therefore the second term has the Z transform:
$$\frac{1}{4} \left( \frac{1}{3} \right)^n u[n-1] \leftrightarrow \frac{1}{12} \cdot \frac{1}{z-\frac{1}{3}}, \quad \text{ROC:} \quad |z| > \frac{1}{3}$$
and the Z transform of the whole input $x[n]$ is:
$$X(z) = \frac{z}{z-\frac{1}{3}} - \frac{1}{12} \cdot \frac{1}{z-\frac{1}{3}} = \frac{z-\frac{1}{12}}{z-\frac{1}{3}}, \quad \text{ROC:} \quad |z| > \frac{1}{3}$$

The Z transform of the output is:
$$Y(z) = \frac{z}{z-\frac{1}{4}}, \quad \text{ROC:} \quad |z| > \frac{1}{4}$$

Therefore the system function is the ratio of the two, and the ROC is the intersection of the ROCs of the two:
$$\begin{aligned}
H(z) = \frac{Y(z)}{X(z)} &= \frac{z}{z-\frac{1}{4}} \cdot \frac{z-\frac{1}{3}}{z-\frac{1}{12}}, \quad \text{ROC:} \quad |z| > \frac{1}{3} \quad \text{and} \quad |z| > \frac{1}{4}\\
&= \frac{z (z-\frac{1}{3})}{(z-\frac{1}{4})(z-\frac{1}{12})}, \quad \text{ROC:} \quad |z| > \frac{1}{3}\\
\end{aligned}$$

The zeros are the roots of the numerator polynomial, i.e. $z_1 = 0$ and $z_2 = \frac{1}{3}$.

The poles are the roots of the denominator polynomial, i.e. $p_1 = \frac{1}{4}$ and $p_2 = \frac{1}{12}$.

The pole-zero diagram is:

![Pole-zero diagram](./img/Ex03_05_01.png){width=75%}

b). *Compute the impulse response $h[n]$ of the system*

We compute $h[n]$ as the inverse Z transform of $H(z)$, using the same method
as in the previous exercises.

The system is causal (it is mentioend in the text, and also because the ROC is the outside of a circle), so $h[n]$ must be causal, which means
we invert the fractions using the variant with $u[n]$ for all fractions.

c). *Find the difference equation of the system*

We disband the parantheses in $H(z)$ and simplify to obtain negative exponents:
$$\begin{aligned}
H(z) &= \frac{z (z-\frac{1}{3})}{(z-\frac{1}{4})(z-\frac{1}{12})} \\
&= \frac{z^2 - \frac{1}{3}z}{z^2 - \frac{4}{12}z + \frac{1}{48}}\\
&= \frac{1 - \frac{1}{3}z^{-1}}{1 - \frac{1}{3}z^{-1} + \frac{1}{48}z^{-2}}
\end{aligned}$$

We can write the system equation directly, knowing that the numerator
coefficients are the coefficients of $x[n-k]$ and the denominator coefficients, with the opposite sign, are the coefficients of $y[n-k]$:
$$y[n] = \frac{1}{3} y[n-1] - \frac{1}{48} y[n-2] + x[n] - \frac{1}{3} x[n-1]$$

We could also take the long route to the same result:
$$H(z) = \frac{1 - \frac{1}{3}z^{-1}}{1 - \frac{1}{3}z^{-1} + \frac{1}{48}z^{-2}} = \frac{Y(z)}{X(z)}$$
$$Y(z) (1 - \frac{1}{3}z^{-1} + \frac{1}{48}z^{-2}) = X(z) (1 - \frac{1}{3}z^{-1})$$
$$y[n] - \frac{1}{3} y[n-1] + \frac{1}{48} y[n-2] = x[n] - \frac{1}{3} x[n-1]$$
$$y[n] = \frac{1}{3} y[n-1] - \frac{1}{48} y[n-2] + x[n] - \frac{1}{3} x[n-1]$$

d). *Characterize the system with respect to those three properties*

1. Since the system function $H(z)$ has a denominator (has poles), it is an IIR system, so the length of the impulse response is infinite.

   We can also see from the expression of $h[n]$ which we obtained in b).

2. The system is recursive, because it has a feedback loop ($y[n]$ depends on $y[n-1]$ and $y[n-2]$ in the equation).

   Any IIR system is recursive.

3. The system is stable, because:

   - it is causal
   - the poles are inside the unit circle ($p_1 = \frac{1}{4}$, $p_2 = \frac{1}{12}$).
